src/GC.fst
@@ -11,35 +11,14 @@ open ExprTypes
 open Interpreter
 
 (* Garbage-collected reversible circuit compilation -- experimental *)
-type qubit =
-  { id   : int;
-    ival : BoolExp;
-    cval : BoolExp }
-
-val null_q    : qubit
-val getSubs   : Total.t int qubit -> Tot (Total.t int int)
-val ids       : Total.t int qubit -> Tot (set int)
-val data_q    : int -> Tot qubit
-val anc_q     : int -> Tot qubit
-//val applyCval : qubit -> Tot qubit
-
-let nullq       = { id = 0; ival = BFalse; cval = BFalse }
-let getSubs     = mapVals (fun q -> q.id)
-let ids m       = vals (getSubs m)
-let data_q i    = { id = i; ival = BVar i; cval = BFalse }
-let anc_q i     = { id = i; ival = BFalse; cval = BFalse }
-//let applyCval q = { id = q.id; ival = q.ival;
 
 type circGCState =
   { top    : int;
     ah     : AncHeap;
     gates  : list Gate;
-    symtab : Total.t int qubit }
-
-val applyCvals : (BoolExp -> Tot BoolExp) -> Total.t int qubit -> Tot (Total.t int qubit)
-let applyCvals f symtab = 
-  let g q = { id = q.id; ival = q.ival; cval = f q.cval } in
-    mapVals g symtab
+    symtab : Total.t int int;
+    ivals  : Total.t int BoolExp;
+    cvals  : Total.t int BoolExp }
 
 val circGC       : circGCState -> int -> Tot circGCState
 val circGCInit   : circGCState
@@ -51,73 +30,83 @@ val circGCEval   : circGCState -> state -> int -> Tot bool
      -compile the current value in place (i.e. ival + cval + cval = ival),
      -if the qubit is an ancilla, push it back onto the heap, and
      -update the current value of all other bits by substituting q.id with ival + cval *)
-val garbageCollect : circGCState -> qubit -> Tot circGCState
-let garbageCollect cs q = 
-  let (ah', res, ancs, circ) = compileBexp cs.ah q.id q.cval in
-  let ah'' = if q.ival = BFalse then insert ah' q.id else ah' in
-  let f bexp = substOneVar bexp q.id (BXor (q.ival, q.cval)) in
-  let symtab' = applyCvals f cs.symtab in
+val garbageCollect : circGCState -> int -> Tot circGCState
+let garbageCollect cs bit = 
+  let ival = lookup cs.ivals bit in
+  let cval = lookup cs.cvals bit in
+  let (ah', res, ancs, circ) = compileBexp cs.ah bit cval in
+  let ah'' = if ival = BFalse then insert ah' bit else ah' in
+  let f bexp = substOneVar bexp bit (BXor (ival, cval)) in
+  let cvals' = mapVals f cs.cvals in
     { top    = cs.top; 
       ah     = ah''; 
       gates  = cs.gates @ circ; 
-      symtab = symtab' }
+      symtab = cs.symtab;
+      ivals  = cs.ivals;
+      cvals  = cvals' }
 
 let circGCInit = 
   { top    = 0; 
     ah     = emptyHeap; 
     gates  = []; 
-    symtab = constMap nullq }
+    symtab = constMap 0;
+    ivals  = constMap BFalse;
+    cvals  = constMap BFalse }
 
 let circGCAlloc cs = 
   let (ah', bit) = popMin cs.ah in
-  let q = { id = bit; 
-	    ival = BFalse; 
-	    cval = BFalse } 
-  in
   let cs' =
-    { top = cs.top + 1;
-      ah = ah';
-      gates = cs.gates;
-      symtab = update cs.symtab cs.top q }
+    { top    = cs.top + 1;
+      ah     = ah';
+      gates  = cs.gates;
+      symtab = update cs.symtab cs.top bit;
+      ivals  = update cs.ivals bit BFalse;
+      cvals  = update cs.cvals bit BFalse }
   in
     (cs.top, cs')
 
 let circGCAssign cs l bexp =
-  let q = lookup cs.symtab l in
-  let bexp' = substVar bexp (getSubs cs.symtab) in
-  let bexpfac = factorAs bexp' q.id in
-  match (q.cval, bexpfac) with
-    | (BFalse, _)      -> // substitute q.id with BFalse, compile in place
-      let bexp'' = substOneVar bexp' q.id BFalse in
-      let (ah', res, ancs, circ) = compileBexp cs.ah q.id bexp'' in
-      let q' = { id = q.id; ival = q.ival; cval = bexp'' } in
-      let f bexp = substOneVar bexp q.id bexp'' in
-      let symtab' = update (applyCvals f cs.symtab) l q' in
-        { top = cs.top; 
-	  ah = ah'; 
-	  gates = cs.gates @ circ; 
-	  symtab = symtab' }
-    | (_, Some bexp'') -> // compile in place, substitute q.id with q.id \oplus bexp''
-      let (ah', res, ancs, circ') = compileBexp cs.ah q.id bexp'' in
-      let q' = { id = q.id; ival = q.ival; cval = BXor (q.cval, bexp'') } in
-      let f bexp = substOneVar bexp q.id (BXor (BVar q.id, bexp'')) in
-      let symtab' = update (applyCvals f cs.symtab) l q' in
-        { top = cs.top; 
-	  ah = ah'; 
-	  gates = cs.gates @ circ'; 
-	  symtab = symtab' }
+  let bit = lookup cs.symtab l in
+  let bexp' = substVar bexp cs.symtab in
+  let bexpfac = factorAs bexp' bit in
+  match (lookup cs.cvals bit, bexpfac) with
+    | (BFalse, _)      -> // substitute bit with BFalse, compile in place
+      let bexp'' = substOneVar bexp' bit BFalse in
+      let (ah', _, _, circ) = compileBexp cs.ah bit bexp'' in
+      let f bexp = substOneVar bexp bit bexp'' in
+      let cvals' = update (mapVals f cs.cvals) bit bexp'' in
+        { top    = cs.top; 
+	  ah     = ah'; 
+	  gates  = cs.gates @ circ; 
+	  symtab = cs.symtab;
+	  ivals  = cs.ivals;
+	  cvals  = cvals'}
+    | (cval, Some bexp'') -> // compile in place, substitute q.id with q.id \oplus bexp''
+      let (ah', _, _, circ') = compileBexp cs.ah bit bexp'' in
+      let f bexp = substOneVar bexp bit (BXor (BVar bit, bexp'')) in
+      let cvals' = update (mapVals f cs.cvals) bit (BXor (cval, bexp'')) in
+        { top    = cs.top; 
+	  ah     = ah'; 
+	  gates  = cs.gates @ circ'; 
+	  symtab = cs.symtab;
+	  ivals  = cs.ivals;
+	  cvals  = cvals'}
     | _                -> // Compile out of place, clean q.id
-      let (ah', res, ancs, circ') = compileBexp_oop cs.ah bexp' in
-      let q' = { id = res; ival = BFalse; cval = bexp' } in
+      let (ah', bit', _, circ') = compileBexp_oop cs.ah bexp' in
+      let symtab' = update cs.symtab l bit' in
+      let ivals' = update cs.ivals bit' BFalse in
+      let cvals' = update cs.cvals bit' bexp' in
       let cs' = 
-	{ top = cs.top; 
-	  ah = ah'; 
-	  gates = cs.gates @ circ'; 
-	  symtab = update cs.symtab l q' } 
+	{ top    = cs.top; 
+	  ah     = ah'; 
+	  gates  = cs.gates @ circ'; 
+	  symtab = symtab';
+	  ivals  = ivals';
+	  cvals  = cvals' } 
       in
-        garbageCollect cs' q
+        garbageCollect cs' bit
 
-let circGCEval cs st i = lookup (evalCirc cs.gates st) (lookup cs.symtab i).id
+let circGCEval cs st i = lookup (evalCirc cs.gates st) (lookup cs.symtab i)
 
 let circGCInterp = {
   alloc = circGCAlloc;
@@ -130,22 +119,26 @@ val allocNcircGC : list GExpr * circGCState -> i:int ->
 let rec allocNcircGC (locs, cs) i =
   if i <= 0 then (List.rev locs, cs)
   else
-    let (ah', res) = popMin cs.ah in
+    let (ah', bit) = popMin cs.ah in
     let cs' = { top = cs.top + 1;
                 ah = ah';
                 gates = cs.gates;
-                symtab = update cs.symtab cs.top (data_q res) }
+                symtab = update cs.symtab cs.top bit;
+		ivals = update cs.ivals bit (BVar bit);
+		cvals = update cs.cvals bit BFalse }
     in
       allocNcircGC (((LOC cs.top)::locs), cs') (i-1)
 
 val allocTycircGC : GType -> circGCState -> Tot (result (GExpr * circGCState))
 let allocTycircGC ty cs = match ty with
   | GBool ->
-    let (ah', res) = popMin cs.ah in
+    let (ah', bit) = popMin cs.ah in
     let cs' = { top = cs.top + 1;
                 ah = ah';
                 gates = cs.gates;
-                symtab = update cs.symtab cs.top (data_q res) }
+                symtab = update cs.symtab cs.top bit;
+		ivals = update cs.ivals bit (BVar bit);
+		cvals = update cs.cvals bit BFalse }
     in
       Val (LOC cs.top, cs')
   | GArray n ->
@@ -153,10 +146,10 @@ let allocTycircGC ty cs = match ty with
       Val (ARRAY locs, st')
   | _ -> Err "Invalid parameter type for circuit generation"
 
-val lookup_Lst_gc : Total.t int qubit -> lst:(list GExpr){isVal_lst lst} -> Tot (list int)
+val lookup_Lst_gc : Total.t int int -> lst:(list GExpr){isVal_lst lst} -> Tot (list int)
 let rec lookup_Lst_gc symtab lst = match lst with
   | [] -> []
-  | (LOC l)::xs -> ((lookup symtab l).id)::(lookup_Lst_gc symtab xs)
+  | (LOC l)::xs -> ((lookup symtab l))::(lookup_Lst_gc symtab xs)
 
 (* Scrubs the state with respect to the remainder of the program
 let findGarbage gexp cs = Set.diff (keys cs.symtab) (locs gexp)
@@ -181,11 +174,11 @@ let rec compileGCCirc (gexp, cs) =
         | Val (v, cs') -> compileGCCirc (substGExpr t x v, cs')
       end
     | LOC l ->
-      let res = lookup cs.symtab l in
-        Val ([res.id], cs.gates)
+      let bit = lookup cs.symtab l in
+        Val ([bit], cs.gates)
     | ARRAY lst ->
-      let res = lookup_Lst_gc cs.symtab lst in
-        Val (res, cs.gates)
+      let bits = lookup_Lst_gc cs.symtab lst in
+        Val (bits, cs.gates)
   else match (step (gexp, cs) circGCInterp) with
     | Err s -> Err s
     | Val c' -> compileGCCirc c'
@@ -199,20 +192,10 @@ let rec compileGCCirc (gexp, cs) =
      - for every active qubit, q.ival = q' <> q.cval' *)
 type validGCState (cs:circGCState) (init:state) =
   zeroHeap (evalCirc cs.gates init) cs.ah /\ 
-  disjoint (ids cs.symtab) (elts cs.ah) /\
-  (forall q. Set.mem q (vals cs.symtab) ==> 
-    evalBexp q.ival init = evalBexp (BXor (BVar q.id, q.cval)) (evalCirc cs.gates init))
-
-val subst_subset_active : cs:circGCState -> bexp:BoolExp ->
-  Lemma (subset (vars (substVar bexp (getSubs cs.symtab))) (ids cs.symtab))
-  (decreases bexp)
-let rec subst_subset_active cs bexp = match bexp with
-  | BFalse -> ()
-  | BVar i -> admit() //lookup_is_val cs.symtab i -- no reason this should fail
-  | BNot x -> subst_subset_active cs x
-  | BAnd (x, y) | BXor (x, y) -> 
-    subst_subset_active cs x;
-    subst_subset_active cs y
+  disjoint (vals cs.symtab) (elts cs.ah) /\
+  (forall bit. Set.mem bit (vals cs.symtab) ==> 
+    evalBexp (lookup cs.ivals bit) init = 
+    evalBexp (BXor (BVar bit, (lookup cs.cvals bit))) (evalCirc cs.gates init))
 
 val valid_alloc : cs:circGCState -> init:state ->
   Lemma (requires (validGCState cs init))
@@ -223,60 +206,51 @@ let valid_alloc cs init =
     pop_proper_subset cs.ah;
     zeroHeap_subset (evalCirc cs.gates init) cs.ah cs'.ah
 
-(* Random lemma about symbol table lookups *)
-val id_is_mem : symtab:t int qubit -> l:int -> 
-  Lemma (Set.mem (lookup symtab l).id (ids symtab))
-  (decreases symtab.elts)
-let rec id_is_mem symtab l = match symtab.elts with
-  | [] -> ()
-  | x::xs -> 
-    let symtab' = { elts = xs; dval = symtab.dval } in
-      id_is_mem symtab' l
-
-val apply_ids_same : f:(BoolExp -> Tot BoolExp) -> symtab:Total.t int qubit  ->
-  Lemma (ids symtab = ids (applyCvals f symtab))
-  (decreases symtab.elts)
-let rec apply_ids_same f symtab = match symtab.elts with
-  | [] -> ()
-  | x::xs -> 
-    let symtab' = { elts = xs; dval = symtab.dval } in
-      apply_ids_same f symtab';
-      admit()
-
 val valid_assign : cs:circGCState -> l:int -> bexp:BoolExp -> init:state ->
   Lemma (requires (validGCState cs init))
 	(ensures  (validGCState (circGCAssign cs l bexp) init))
 let valid_assign cs l bexp init =
-  let q = lookup cs.symtab l in
-  let bexp' = substVar bexp (getSubs cs.symtab) in
-  let bexpfac = factorAs bexp' q.id in
+  let bit = lookup cs.symtab l in
+  let bexp' = substVar bexp cs.symtab in
+  let bexpfac = factorAs bexp' bit in
   let cs' = circGCAssign cs l bexp in
-  match (q.cval, bexpfac) with
+  let st = evalCirc cs.gates init in
+  let st' = evalCirc cs'.gates init in
+  match (lookup cs.cvals bit, bexpfac) with
     | (BFalse, _)      -> 
-      let bexp'' = substOneVar bexp' q.id BFalse in
-      let (ah', res, ancs, circ) = compileBexp cs.ah q.id bexp'' in
-      let q' = { id = q.id; ival = q.ival; cval = bexp'' } in
-      let f bexp = substOneVar bexp q.id bexp'' in
-	substVar_elems bexp (getSubs cs.symtab); // subset (vars bexp') (ids cs.symtab)
-	substOneVar_elems bexp' q.id BFalse;     // subset (vars bexp'') (vars bexp' \ q.id)
-	id_is_mem cs.symtab l;                   // q.id in ids (symtab)
-	compile_bexp_zero cs.ah q.id bexp'' (evalCirc cs.gates init);
+      let bexp'' = substOneVar bexp' bit BFalse in
+      let (ah', _, _, circ) = compileBexp cs.ah bit bexp'' in
+      let f bexp = substOneVar bexp bit bexp'' in
+	substVar_elems bexp cs.symtab;      // subset (vars bexp') (vals cs.symtab)
+	substOneVar_elems bexp' bit BFalse; // subset (vars bexp'') (vars bexp' \ bit)
+	lookup_is_val cs.symtab l;          // bit in (vals symtab)
+	compile_bexp_zero cs.ah bit bexp'' st;
 	//admitP(zeroHeap (evalCirc cs'.gates init) cs'.ah);
-	compile_decreases_heap cs.ah q.id bexp''; // subset cs.ah' cs.ah
-	disjoint_subset (elts ah') (elts cs.ah) (ids cs.symtab); // disjoint cs.ah' (ids cs.symtab)
-	apply_ids_same f cs.symtab;
-	//assert(ids cs'.symtab = ins q.id (ids (applyCvals f cs.symtab)));
-	admit();
+	compile_decreases_heap cs.ah bit bexp'';                  // subset cs.ah' cs.ah
+	disjoint_subset (elts ah') (elts cs.ah) (vals cs.symtab); // disjoint cs.ah' (ids cs.symtab)
 	//admitP(disjoint (ids cs'.symtab) (elts cs'.ah));
-	admitP(forall q. Set.mem q (vals cs'.symtab) ==> 
-	  evalBexp q.ival init = evalBexp (BXor (BVar q.id, q.cval)) (evalCirc cs'.gates init))
+	compile_bexp_correct cs.ah bit bexp'' st; // lookup bit st' = lookup bit st <> evalBexp bexp'' st 
+	compile_mods cs.ah bit bexp'';            // subset (mods circ) (ins bit (elts cs.ah))
+	eval_mod st circ;                         // agree_on st st' complement (mods circ)
+	eval_state_swap bexp'' st st';            // evalBexp bexp'' st = evalBexp bexp'' st'
+	admitP(b2t(evalBexp (BXor (BVar bit, (lookup cs.cvals bit))) st =
+	           evalBexp (BXor (BVar bit, (lookup cs'.cvals bit))) st'));
+	disjoint_is_subset_compl (rem bit (vals cs'.symtab)) (ins bit (elts cs.ah));
+	subset_compl_reverse (mods circ) (ins bit (elts cs.ah));
+	subset_trans (rem bit (vals cs'.symtab)) (complement (ins bit (elts cs.ah))) (complement (mods circ));
+	agree_on_subset st st' (complement (mods circ)) (rem bit (vals cs'.symtab));
+	//assert(forall b. (Set.mem b (rem bit (vals cs'.symtab))) ==> evalBexp (BVar b) st = evalBexp (BVar b) st');
+	//assert(agree_on st st' (rem bit (vals cs'.symtab))); 
+	admitP(forall b. (Set.mem b (vals cs'.symtab) /\ not (b = bit)) ==> 
+	  evalBexp (BXor (BVar b, (lookup cs.cvals b))) (evalCirc cs.gates init) =
+	  evalBexp (BXor (BVar b, (lookup cs'.cvals b))) (evalCirc cs'.gates init))
     | (_, Some bexp'') ->
 	admitP(validGCState cs' init) (*
 	admitP(zeroHeap (evalCirc cs'.gates init) cs'.ah);
 	admitP(disjoint (ids cs'.symtab) (elts cs'.ah));
 	admitP(forall q. Set.mem q (vals cs'.symtab) ==> 
 	  evalBexp q.ival init = evalBexp (BXor (BVar q.id, q.cval)) (evalCirc cs'.gates init))*)
-    | _                -> 
+    | _                ->
 	admitP(validGCState cs' init)(*
 	admitP(zeroHeap (evalCirc cs'.gates init) cs'.ah);
 	admitP(disjoint (ids cs'.symtab) (elts cs'.ah));
